cbn.v
@@ -21,8 +21,8 @@ Definition I (e : tm ) : configuration := st nil e.
 (* Direct description of Maraist et al. Figure 8, with amendment from  *)
 Reserved Notation " c1 '⇓' c2 " (at level 50).
 Inductive step : configuration → configuration → Prop :=
-  | Id : ∀ M N y x Φ Ψ Υ, ⟨Φ, x ↦ M, Υ⟩M ⇓ ⟨Ψ, x ↦ M, Υ⟩:λy,N →
-            ⟨Φ, x ↦ M, Υ⟩var x ⇓ ⟨Ψ, x ↦ :λy,N, Υ⟩:λy,N
+  | Id : ∀ M N y x Φ Υ Φ' Υ', ⟨Φ, x ↦ M, Υ⟩M ⇓ ⟨Φ', x ↦ M, Υ'⟩:λy,N →
+            ⟨Φ, x ↦ M, Υ⟩var x ⇓ ⟨Φ', x ↦ :λy,N, Υ'⟩:λy,N
   | Abs : ∀ N x Φ,  ⟨Φ⟩:λx,N ⇓ ⟨Φ⟩:λx,N
   | App : ∀ M N L B y x x' Φ Ψ Υ,
               fresh' x' Ψ → 
@@ -103,12 +103,28 @@ assumption. simpl. simpl in H3. destruct H3. assert (subset (fvs ([x' // x]N))
 (cons_subset x') in H3. apply subset_trans with (ys:=x'::remove x (fvs N)).
 assumption. assumption. Qed. 
 
+Lemma unique_inf_eq {A B} : ∀ (Φ Φ' Ψ Ψ' : list (prod A B)) c, 
+  unique (domain (Φ ++ c :: Ψ)) → 
+  unique (domain (Φ' ++ c :: Ψ')) →
+  Φ ++ c :: Ψ = Φ' ++ c :: Ψ' →
+  Φ = Φ' ∧ Ψ = Ψ'. 
+induction Φ; intros; destruct c. inversion H. subst. induction Φ'. simpl in H1.
+inversion H1. subst. auto. destruct a0. simpl in H1. subst. inversion H1. subst.
+inversion H0. subst. specialize (H6 (inf_indomain _ _ _ _)). inversion H6.
+induction Φ'. inversion H1. subst. inversion H. subst. specialize (H4
+(inf_indomain _ _ _ _)). inversion H4. inversion H1. subst. simpl in H1. 
+simpl in H0. inversion H0. subst. inversion H. subst. 
+specialize (IHΦ Φ' _ Ψ' _ H8 H6 H4). destruct IHΦ. subst. auto. Qed. 
+
 Lemma det_step : ∀ a b c, well_formed a → a ⇓ b → a ⇓ c → b = c. 
-intros a b c wf s. generalize dependent c. induction s. apply well_formed_app in
-wf. specialize (IHs wf). intros. inversion H. subst. symmetry in H0. apply
+intros a b c wf s. generalize dependent c. induction s. assert (wfx := wf).
+apply well_formed_app in wf.  intros. inversion H. subst. symmetry in H0. apply
 unique_inf in H0; try (destruct wf; destruct H2; assumption). destruct H0.
-destruct H1. subst. apply IHs in H3. inversion H3. subst. apply app_eq_l in H1.
-inversion H1.  subst. reflexivity. intros. inversion H. subst. auto. inversion 
+destruct H1. subst. apply IHs in H3. inversion H3. apply unique_inf_eq
+in H1. destruct H1. subst. reflexivity. subst. set (wf' := well_formed_step _ _
+wf s). unfold well_formed in wf'. destruct wf'. destruct H2. assumption. subst.
+rewrite H1 in s.  set (wf' := well_formed_step _ _ wf s). destruct wf'. destruct
+H2. assumption. assumption. intros. inversion H. subst. auto. inversion 
 wf. simpl in H0. rewrite app_subset_and in H0. destruct H0. specialize (IHs1
 (conj H0 H1)). assert (s1':=s1). apply well_formed_step in s1; try (apply (conj
 H0 H1)). destruct s1. assert (s1:=s1'). simpl in H3. apply monotonic_heap in s1.
@@ -153,3 +169,113 @@ H2. simpl. destruct H2. unfold closed_under in H0. rewrite <- subset_eq in H0.
 apply H0 in H2. apply H3 in H2. assumption. Qed. 
 
 *)
+
+Inductive reachable (h : heap) : nat → tm → Prop := 
+  | rchi : ∀ x e, In x (fvs e) →  reachable h x e
+  | rchtran : ∀ x y e e', reachable h x e → 
+                           lookup x h = Some e' → 
+                           In y (fvs e') → 
+                           reachable h y e.
+
+Lemma rchapp : ∀ h x y e e', reachable h x e → 
+                              lookup x h = Some e' → 
+                              reachable h y e' → 
+                              reachable h y e.
+intros. induction H1. apply rchtran with (x:=x) (e':=e0); assumption. apply
+IHreachable in H0. apply rchtran with (x:=x0) (e':=e'). assumption.
+assumption. assumption. Qed.
+
+Lemma rchtran' : ∀ h x y e e', In x (fvs e) →
+                                lookup x h = Some e' →
+                                reachable h y e' →
+                                reachable h y e. 
+intros. induction H1. apply rchi with (h:=h) in H. apply rchtran with (x:=x)
+(e':=e0). assumption. assumption. assumption. apply rchi with (h:=h) in H3.
+apply rchapp with (x:=x0) (e':=e'); try auto. Qed.  
+
+Lemma rchdestruct : ∀ h l e, reachable h l e → 
+  In l (fvs e) ∨ 
+  ∃ (e':tm) (x:nat), In x (fvs e) ∧ lookup x h = Some e' ∧ reachable h l e'. 
+intros. prep_induction H. induction H; intros; auto; subst. destruct
+IHreachable. apply or_intror. exists e', x. split; try auto. split; try
+auto. apply rchi with (h:=h) in H1. assumption. destruct H2. destruct H2.
+destruct H2. destruct H3. assert (cbn0 := rchtran _ _ _ _ _ H4 H0 H1). apply
+or_intror. exists x0, x1; split; try auto.  Qed.  
+
+Definition acyclic (Φ : heap) : Prop := forevery Φ (λ x, 
+  match x with (l, e) => ¬ reachable Φ l e end). 
+
+Lemma reachable_app : ∀ l Φ Ψ c, unique (domain (Ψ ++ Φ)) → 
+  reachable (Φ ++ Ψ) l c → reachable (Ψ ++ Φ) l c. 
+intros. induction H0. apply rchi. assumption. apply rchtran with (x:=x)
+(e':=e'). assumption. rewrite lookup_app_unique. assumption. assumption.
+assumption. Qed.  
+
+(* Decidable reachability, not currently used *)
+Definition reachables (h : heap) (e : tm) := 
+let h' := concat (map (const h) h) in 
+  (fix f l acc := match l with
+  | nil => acc
+  | cons (n, e) t => f t (if in_dec eq_nat_dec n acc then (fvs e ++ acc) else acc)
+  end) h (fvs e).
+
+(* reachability dependent *)
+Lemma dup_irrelevent : ∀ l l' h  h' e,
+  unique (domain (h ++ (l, e) :: h')) →
+  reachable (h ++ (l, e) :: h') l' e →
+  reachable (h ++ h') l' e.
+intros. prep_induction H0. induction H0; intros; subst. apply
+rchi. assumption. specialize (IHreachable l h h' H3 eq_refl). destruct
+(eq_nat_dec x l). subst. rewrite lookup_inf in H. inversion H. subst. apply
+rchi. assumption. assumption. apply rchtran with (x:=x) (e':=e'). assumption.
+apply lookup_not_inf with (a:=e) (h0:=h) (h'0:=h') in n. rewrite <- n.
+assumption. assumption. Qed.
+
+Lemma reachable_cons : ∀ b h l e, unique (domain (b::h)) → reachable h l e → reachable (b::h)
+l e. intros. induction H0. apply rchi. assumption. apply rchtran with (x:=x)
+(e':=e'). assumption. unfold lookup. simpl. destruct b. simpl. destruct (beq_nat
+x n) eqn:bxn. apply beq_nat_true in bxn. subst.  simpl in H. inversion H. subst. 
+apply lookup_domain in H1. apply H5 in H1. inversion H1. assumption. assumption.
+Qed. 
+
+Lemma reachable_or_app : ∀ h l m n, (reachable h l m ∨ reachable h l n) → 
+  reachable h l (app m n). 
+intros. destruct H; induction H. apply rchi. simpl. apply in_or_app. apply
+or_introl. assumption. apply rchtran with (x:=x) (e':=e'); try auto. apply
+rchi. simpl. apply in_or_app. apply or_intror. assumption. apply rchtran with
+(x:=x) (e':=e'); try auto. Qed. 
+
+Lemma reachable_app_or : ∀ h l m n, reachable h l (app m n) →
+  reachable h l m ∨ reachable h l n. 
+intros. prep_induction H. induction H; intros; subst. simpl in H. apply in_app_or in H. destruct H.
+apply or_introl. apply rchi. assumption. apply or_intror. apply rchi.
+assumption. specialize (IHreachable m n eq_refl). destruct IHreachable.
+apply or_introl. apply rchtran with (x:=x) (e':=e'); try auto. apply or_intror.
+apply rchtran with (x:=x) (e':=e'); try auto. Qed. 
+
+Lemma reachable_app_iff : ∀ h l m n, reachable h l m ∨ reachable h l n 
+                                       ↔ reachable h l (app m n). 
+split. apply reachable_or_app. apply reachable_app_or. Qed.
+
+Lemma unreachable_app : ∀ h l m n, ¬ reachable h l (app m n) → ¬
+reachable h l m ∧ ¬ reachable h l n. 
+intros. split. unfold not. intros. apply or_introl with
+(B:=reachable h l n) in H0. apply reachable_or_app in H0. apply H in H0.
+assumption. unfold not. intros. apply or_intror with (A:=reachable h l m)in
+H0. apply reachable_or_app in H0. apply H in H0. assumption. Qed. 
+
+Definition substep 
+
+Lemma heap_reachable_step : ∀ Φ Ψ m v l e, step (st Ψ m) (st Φ v) →
+                                           lookup l Ψ = Some e →
+                                           ∃ e', lookup l Φ = Some e' ∧  
+                                           (e' = e ∨ step (st Φ e) (st Φ e')). 
+intros. prep_induction H. induction H; intros; subst. inversion H3. inversion
+H2. subst. clear H2. clear H3.  specialize (IHstep _ _ _ _ _ _ H0 eq_refl
+eq_refl). destruct IHstep. destruct H1. destruct H2. subst. destruct
+(eq_nat_dec l x). subst. rewrite lookup_inf.   
+inversion H2. inversion H1. subst. clear H1. clear H2. rewrite
+forevery_app in IHstep. destruct IHstep. simpl in H1. destruct H1. destruct H1.
+destruct H1. destruct H1. rewrite forevery_app. split.  
+
+
