cbn_cem.v
@@ -1,9 +1,10 @@
 Require cem cbn expr db relations.
 Require Import Minus.
 Require Import Unicode.Utf8 List NaryFunctions.
-Require Import expr_db util CpdtTactics.
+Require Import expr_db util CpdtTactics JRWTactics.
 Require Import Basics EqNat.
 Require Import Compare_dec.
+Require Import Arith.Peano_dec.
 
 Open Scope program_scope. 
 
@@ -28,54 +29,11 @@ Fixpoint etolg (e : expr.tm) (env : Map nat nat) :=  match e with
     end
   end.
  
-Definition fmap_option {a b} : (a → b) → option a → option b := λ f o, 
-  match o with 
-  | Some m => Some (f m)
-  | None => None
-  end.
-
-Definition seq_option {a b} : option (a → b) → option a → option b := λ f o,
-  match f, o with
-    | Some g, Some a => Some (g a)
-    | _, _ => None
-  end.
-  
-Notation "f <$> x" := (fmap_option f x) (at level 30).
-Notation "f <*> x" := (seq_option f x) (at level 40).
-
 Fixpoint cte (t:db.tm) (d:nat) : lgexpr := match t with
   | db.lam b => lam (cte b (S d))
   | db.app m n => app (cte m d) (cte n d)
   | db.var v => if gt_dec d v then lvar v else gvar (v-d)
   end.
-
-Fixpoint fvs' (t:db.tm) (d:nat) : list nat := match t with
-  | db.lam b => fvs' b (S d)
-  | db.app m n => fvs' m d ++ fvs' n d
-  | db.var v => if gt_dec d v then nil else (v-d)::nil
-  end.
-
-Lemma filter_app {A} : ∀ xs ys (p:A → bool), filter p xs ++ filter p ys = filter p (xs ++ ys). 
-intros. induction xs. reflexivity. simpl. destruct (p a). simpl. 
-rewrite <- IHxs. reflexivity. apply IHxs. Qed. 
-
-Lemma fvs_eq : ∀ t d, map (λ x, x - d) (filter (λ x, if gt_dec d x then false
-else true) (db.fvs t)) = fvs' t d.
-intros t. induction t; intros. simpl. destruct (gt_dec d n). reflexivity. simpl.
-reflexivity. simpl. assert (∀ xs d, map (λ x : nat, x - S d) (filter (λ x : nat, if gt_dec
-(S d) x then false else true) xs) = map (λ x :
-nat, x - d) (filter (λ x : nat, if gt_dec d x then false else true) (map pred
-(remove 0 xs)))). intros. induction xs. reflexivity. destruct a. simpl. apply
-IHxs. simpl. destruct (gt_dec d0 a). apply Gt.gt_n_S in g. destruct (gt_dec (S
-d0) (S a)). apply IHxs. apply n in g. inversion g. destruct (gt_dec (S d0) (S
-a)). apply Gt.gt_S_n in g. apply n in g. inversion g. simpl. rewrite IHxs.
-reflexivity. specialize IHt with (S d). rewrite <- IHt. rewrite H. reflexivity.
-simpl. rewrite <- IHt1. rewrite <- IHt2. rewrite <- map_app. rewrite <-
-filter_app. reflexivity. Qed. 
-
-Lemma fvs_eq_zero : ∀ t, db.fvs t = fvs' t 0.
-intros. rewrite <- fvs_eq. simpl. induction (db.fvs t). simpl. reflexivity. 
-simpl. rewrite <- minus_n_O. rewrite <- IHl. reflexivity. Qed. 
 
 Fixpoint gfvs (t:lgexpr) : list nat := match t with
   | lam b => gfvs b
@@ -84,7 +42,7 @@ Fixpoint gfvs (t:lgexpr) : list nat := match t with
   | lvar v => nil
   end.
 
-Lemma gfvs_fvs : ∀ t d, gfvs (cte t d) = fvs' t d.
+Lemma gfvs_fvs : ∀ t d, gfvs (cte t d) = db.fvs' t d.
 intros t. induction t; intros. simpl. destruct (gt_dec d n). reflexivity. reflexivity.
 apply IHt. simpl. rewrite IHt1. rewrite IHt2. reflexivity. Qed.
 
@@ -97,7 +55,7 @@ Lemma forevery_subset {A} : ∀ xs ys (p:A→Prop), xs ⊆ ys → forevery ys p 
 intros. induction xs. auto. simpl. simpl in H. destruct H. apply IHxs in H1.
 split. apply (forevery_in _ _ _ H H0). assumption. Qed.
 
-Lemma cte_lu : ∀ t d v, cte t d = gvar (d-v) → In (d-v) (fvs' t d). 
+Lemma cte_lu : ∀ t d v, cte t d = gvar (d-v) → In (d-v) (db.fvs' t d). 
 intros. destruct t; inversion H. simpl. destruct (gt_dec d n). inversion H1. inversion
 H1. rewrite H2. simpl. apply (or_introl eq_refl). Qed. 
 
@@ -120,7 +78,7 @@ reflexivity. induction v. rewrite <- Heqo in H. inversion H. rewrite <- Heqo in
 H. inversion H. Qed.
 
 Definition closed_up_to (c:cem.closure) (h:cem.heap) (d:nat) : Prop := match c with
-  | cem.close t e => forevery (fvs' t d) (λ x, ∃ e' c', cem.clu x e h = Some (e',c') ∧ In e' (domain h))
+  | cem.close t e => forevery (db.fvs' t d) (λ x, ∃ e' c', cem.clu x e h = Some (e',c') ∧ In e' (domain h))
   end.  
 
 Lemma closed_to_lg : ∀ t e h d, closed_up_to (cem.close t e) h d → ∃ e', 
@@ -139,7 +97,7 @@ rewrite H. rewrite H0. reflexivity. Qed.
 
 Lemma wf_to_lg : ∀ c, cem.well_formed c → ∃ e, conftolg c 0 = Some e.
 intros. destruct c. destruct H. unfold cem.closed_under in H. destruct st_clos.
-rewrite fvs_eq_zero in H. apply closed_to_lg in H. assumption. Qed. 
+rewrite db.fvs_eq_zero in H. apply closed_to_lg in H. assumption. Qed. 
 
 Record configuration := conf {
   st_heap : Map nat lgexpr;
@@ -149,57 +107,15 @@ Record configuration := conf {
 Definition eq_terms (t:expr.tm) (c:cem.configuration) : Prop := 
   Some (etolg t nil) = conftolg c 0.
 
-Definition equal_heaps (h : cem.heap) (h' : cbn.heap) := related_lists (λ x y, match x,y with
+Definition eq_heaps (h : cem.heap) (h' : cbn.heap) := related_lists (λ x y, match x,y with
   | (l, cem.cl c e), (l', t) => l = l' ∧ eq_terms t (cem.conf h c)
   end) h h'.
 
 Definition eq_confs (c: cem.configuration) (c':cbn.configuration) : Prop := 
   cem.well_formed c ∧ cbn.well_formed c' ∧ 
   match c, c' with
-  | cem.conf h cl, cbn.st h' e' => eq_terms e' c ∧ equal_heaps h h'
+  | cem.conf h cl, cbn.st h' e' => eq_terms e' c ∧ eq_heaps h h'
   end.
-
-Lemma expr_closed_under_db: ∀ t xs, expr.fvs t ⊆ domain xs → {e | db t xs = Some e}.
-intros t. induction t; intros; simpl in H. destruct H. simpl.
-apply in_domain_lookup in H.  destruct H. rewrite e. exists (db.var x).
-reflexivity. 
-
-rewrite app_subset_and in H. destruct H. apply IHt1 in H. apply IHt2 in H0.
-destruct H.  destruct H0. simpl. rewrite e. rewrite e0. exists (db.app x x0).
-reflexivity.   
-
-simpl in H. rewrite <- subset_remove_cons in H. rewrite <- domain_fmap with
-(f:=S) in H.  specialize (IHt ((n,0)::map (fmap S) (xs))). simpl in IHt.  apply
-IHt in H. simpl. destruct H. rewrite e. exists (db.lam x). reflexivity. Qed.
-
-Lemma expr_db_closed_under : ∀ t xs e, db t xs = Some e → expr.fvs t ⊆ domain xs. 
-intros t. induction t; intros; simpl in H.
-
-destruct (lookup n xs) eqn:Heqo. apply lookup_domain in Heqo. simpl. split;
-auto. inversion H. 
-
-simpl. destruct (db t1 xs) eqn:Heqo. destruct (db t2 xs)
-eqn:Heqo0. apply IHt1 in Heqo. apply IHt2 in Heqo0. rewrite app_subset_and; 
-split; auto. inversion H. inversion H. 
-
-specialize (IHt ((n,0)::map (fmap S) xs)). destruct (db t ((n,0)::map (fmap S)
-xs)) eqn:Heqo. inversion H. subst. symmetry in Heqo. specialize (IHt t0
-eq_refl). simpl. simpl in IHt. rewrite domain_fmap in IHt. rewrite <-
-subset_remove_cons.  assumption.  inversion H. Qed.
-
-Lemma expr_db_closed : ∀ t e xs, db t xs = Some e → db.fvs e ⊆ codomain xs. 
-intros t. induction t; intros. inversion H. destruct (lookup n xs). inversion
-H1. subst. simpl. split; auto. unfold codomain. inversion H. remember (lookup n
-xs). destruct o. symmetry in Heqo. apply lookup_codomain in Heqo. inversion H2.
-subst. assumption. inversion H2. inversion H1. simpl in H. remember (db t1 xs).
-remember (db t2 xs). destruct o. destruct o0. symmetry in Heqo. symmetry in
-Heqo0. apply IHt1 in Heqo. apply IHt2 in Heqo0. inversion H. subst. simpl.
-rewrite app_subset_and. split; auto. inversion H. inversion H. inversion H.
-remember (db t ((n,0) :: map (fmap S) xs)). destruct o. symmetry in Heqo. apply
-IHt in Heqo. inversion H1. subst. simpl. simpl in Heqo. unfold codomain in Heqo.
-rewrite map_map in Heqo. rewrite subset_remove_cons in Heqo. apply subset_map with
-(f:=pred) in Heqo. rewrite map_map in Heqo. simpl. rewrite (map_homo _ _
-snd_fmap) in Heqo. assumption. inversion H1. Qed. 
 
 Fixpoint depth_env (xs : list nat) (y : nat) := match xs with 
   | nil => y
@@ -249,7 +165,7 @@ apply unil. split. simpl. apply expr_db_closed_under in H. assumption. split.
 apply unil. simpl. auto. apply expr_db_eq in H. simpl. unfold eq_terms. rewrite
 <- H. simpl. split. reflexivity. apply rel_nil. Qed.  
 
-Lemma equal_heaps_domains : ∀ h h', equal_heaps h h' → domain h = domain h'. 
+Lemma eq_heaps_domains : ∀ h h', eq_heaps h h' → domain h = domain h'. 
 intros. induction H. reflexivity. destruct x. destruct c. destruct y. destruct
 H. subst. simpl. f_equal. assumption. Qed.
 
@@ -270,16 +186,465 @@ clu_some_lu in h'. destruct h'. unfold cem.clu in H. rewrite H0 in H. destruct
 x0. apply IHx in H. destruct H. destruct H. destruct H. subst. exists x0, x1,
 x2.  reflexivity. Qed. 
 
+Lemma related_lists_app {a b} : ∀ (r:relation a b) xs xs' ys ys', 
+  related_lists r xs ys → 
+  related_lists r xs' ys' → 
+  related_lists r (xs ++ xs') (ys ++ ys'). 
+intros. induction H. assumption. simpl. constructor; assumption. Qed.  
+
+Lemma related_lists_app1 {a b} : ∀ (r:relation a b) xs xs' ys ys', 
+  related_lists r (xs ++ xs') (ys ++ ys') →
+  related_lists r xs ys →
+  related_lists r xs' ys'. 
+intros. induction H0. assumption. simpl in H. inversion H. subst. apply
+IHrelated_lists in H7. assumption. Qed. 
+
+Lemma cons_eq_app {A} : ∀ (x:A) xs x1 x2, x :: xs = x1 ++ x2 → 
+  (∃ x1', x1 = x::x1' ∧ xs = x1' ++ x2) ∨
+  (x1 = nil ∧ x2 = x::xs). 
+intros. destruct x1. apply or_intror. auto. apply or_introl. exists x1.
+inversion H. subst. auto. Qed. 
+
+Lemma related_lists_inj_tail {a b} : ∀ (r : relation a b) xs x ys y, 
+  related_lists r (xs ++ x :: nil) (ys ++ y :: nil) →
+  related_lists r xs ys ∧ r x y.
+intros. prep_induction H. induction H; intros. apply app_cons_not_nil in H2.
+inversion H2. destruct ys0. inversion H2. subst. destruct xs0. inversion H1.
+subst. auto. inversion H1. subst. inversion H0. apply app_cons_not_nil in H4.
+inversion H4. inversion H2. subst. destruct xs0. inversion H1. subst. inversion
+H0. apply app_cons_not_nil in H3. inversion H3. inversion H1. subst. specialize
+(IHrelated_lists xs0 x0 ys0 y0 eq_refl eq_refl). destruct IHrelated_lists.
+split; auto. constructor; auto. Qed. 
+
+Lemma related_lists_app2 {a b} : ∀ (r:relation a b) xs xs' ys ys', 
+  related_lists r (xs ++ xs') (ys ++ ys') →
+  related_lists r xs' ys' → 
+  related_lists r xs ys.
+intros. prep_induction H0. induction H0; intros. rewrite app_nil_r in H. rewrite app_nil_r in H.
+assumption. assert (∀ a ys (y:a) ys0, ys ++ y :: ys0 = (ys ++ y :: nil) ++ ys0).
+intros. rewrite <- app_assoc. reflexivity. rewrite (H2 a) in H1. rewrite (H2 b)
+in H1. apply IHrelated_lists in H1.  apply related_lists_inj_tail in H1.
+destruct H1. auto. Qed. 
+
+Lemma not_in_cons {a} : ∀ (x:a) y xs, ¬ In x (y::xs) ↔ y ≠ x ∧ ¬ In x xs. 
+intros. split. split; unfold not; intros. apply or_introl with (B:=In x xs) in H0.
+simpl in H. apply H in H0. assumption. apply or_intror with (A:=y = x) in H0.
+apply H in H0. assumption. intros. unfold not; intros. destruct H. simpl in H0.
+destruct H0. apply H in H0. assumption. apply H1 in H0. assumption. Qed.
+
+Lemma not_in_app {a} : ∀ (x:a) xs ys, ¬ In x (xs ++ ys) ↔ ¬ In x xs ∧ ¬ In x ys. 
+intros. split. split; unfold not; intros. apply or_introl with (B:=In x ys) in H0.
+apply in_or_app in H0. apply H in H0. assumption. apply or_intror with (A:=In x
+xs) in H0. apply in_or_app in H0. apply H in H0. assumption. intros. unfold not.
+intros. destruct H. apply in_app_or in H0. destruct H0. auto. auto. Qed.  
+
+Lemma unique_app {a} : ∀ (xs:list a) ys, unique (xs ++ ys) → unique xs ∧ unique ys. 
+intros. induction xs. split; auto. constructor. simpl in H. inversion H. subst.
+apply IHxs in H3. destruct H3. split; auto. constructor. apply not_in_app in H2.
+destruct H2. assumption. assumption. Qed. 
+
+Lemma unique_inj_last {a} : ∀ xs (x:a),¬ In x xs → unique xs → unique (xs ++ x :: nil). 
+induction xs; intros. simpl. constructor. assumption.
+constructor. simpl. apply not_in_cons in H. destruct H. apply IHxs in H1.
+inversion H0. subst. constructor. apply not_in_app. split. assumption. simpl.
+unfold not. intros. destruct H2. symmetry in H2. apply H in H2. auto. auto.
+assumption. inversion H0. assumption. Qed. 
+
+Lemma unique_app_comm {a} : ∀ (xs ys : list a), unique (xs ++ ys) → 
+  unique (ys ++ xs). 
+induction xs; intros. rewrite app_nil_r. auto. simpl in H. inversion H. subst.
+assert (a0 :: xs = (a0 :: nil) ++ xs). reflexivity.  rewrite H0. rewrite
+app_assoc. apply IHxs. rewrite app_assoc. apply unique_inj_last; assumption.
+Qed. 
+
+Lemma related_lists_in {a b} : ∀ (r: relation a b) xs ys x,
+  related_lists r xs ys →
+  In x xs →
+  ∃ y, In y ys ∧ r x y.
+intros. prep_induction H. induction H; intros. inversion H0. simpl in H1.
+destruct H1. subst. exists y. split; auto. simpl. auto. apply IHrelated_lists in
+H1. destruct H1. destruct H1. exists x1. split. simpl. auto. auto. Qed. 
+
+Lemma related_lists_in' {a b} : ∀ (r: relation a b) xs ys y,
+  related_lists r xs ys →
+  In y ys →
+  ∃ x, In x xs ∧ r x y.
+intros. prep_induction H. induction H; intros. inversion H0. simpl in H1.
+destruct H1. subst. exists x. split; auto. simpl. auto. apply IHrelated_lists in
+H1. destruct H1. destruct H1. exists x0. split. simpl. auto. auto. Qed. 
+
+Lemma unique_inf_not_in {a} : ∀ xs ys (l:a), 
+  unique (xs ++ l :: ys) →
+  ¬ In l xs ∧ ¬ In l ys. 
+intros. apply unique_app_comm in H. simpl in H. inversion H. subst.
+apply not_in_app in H2. destruct H2. auto. Qed.  
+
+Lemma related_lists_inf {a b} : ∀ (r : relation a b) xs xs' ys ys' x y,
+  related_lists r (xs ++ x :: xs') (ys ++ y :: ys') →
+  (¬ ∃ y, In y ys ∧ r x y) ∧ (¬ ∃ y, In y ys' ∧ r x y) →
+  r x y.
+intros. assert (In x (xs ++ x :: xs')). apply in_inf. apply (related_lists_in _
+_ _ _ H) in H1. destruct H1. destruct H1. destruct H0. apply in_app_or in H1.
+destruct H1. specialize (H0 (ex_intro _ x0 (conj H1 H2))).  inversion H0.
+simpl in H1. destruct H1. subst. assumption. specialize (H3 (ex_intro _ x0 (conj
+H1 H2))). inversion H3. Qed. 
+
+Lemma eq_terms_cons : ∀ xs c c' f d t, isfresh xs f → 
+  conftolg (cem.conf xs c) d = Some t →
+  conftolg (cem.conf ((f, c')::xs) c) d = Some t. 
+destruct c. generalize dependent xs. generalize dependent clos_env. induction
+clos_tm; intros. simpl. simpl in H0. destruct (gt_dec d n). assumption.
+destruct (cem.clu (n-d) clos_env xs) eqn:clue. rewrite <- H0. f_equal. destruct
+c'. apply cem.clu_cons; assumption. inversion H0. simpl. simpl in H0. simpl in
+IHclos_tm. destruct ((fix cte' (t0 : lgexpr) : option lgexpr :=
+        match t0 with
+        | gvar v => (gvar ∘ fst (B:=cem.closure)) <$> cem.clu v clos_env xs
+        | lvar v => Some (lvar v)
+        | lam b => lam <$> cte' b
+        | app m n => app <$> cte' m <*> cte' n
+        end) (cte clos_tm (S d))) eqn:bod. specialize (IHclos_tm clos_env xs c'
+f (S d) l H bod). rewrite IHclos_tm. assumption. inversion H0. simpl. simpl in
+H0. 
+destruct ((fix cte' (t0 : lgexpr) : option lgexpr :=
+        match t0 with
+        | gvar v => (gvar ∘ fst (B:=cem.closure)) <$> cem.clu v clos_env xs
+        | lvar v => Some (lvar v)
+        | lam b => lam <$> cte' b
+        | app m n => app <$> cte' m <*> cte' n
+        end) (cte clos_tm1 d)) eqn:t1e. 
+destruct ((fix cte' (t0 : lgexpr) : option lgexpr :=
+        match t0 with
+        | gvar v => (gvar ∘ fst (B:=cem.closure)) <$> cem.clu v clos_env xs
+        | lvar v => Some (lvar v)
+        | lam b => lam <$> cte' b
+        | app m n => app <$> cte' m <*> cte' n
+        end) (cte clos_tm2 d)) eqn:t2e. 
+specialize (IHclos_tm1 clos_env xs c' f d l H t1e). 
+specialize (IHclos_tm2 clos_env xs c' f d l0 H t2e). simpl in IHclos_tm1. simpl
+in IHclos_tm2. rewrite IHclos_tm1. rewrite IHclos_tm2. assumption. inversion H0.
+inversion H0. Qed.  
+
+Lemma eq_confs_inf : ∀ x x' l m c e y y' m' c', 
+  eq_confs (cem.conf (x' ++ (l, cem.cl c e) :: y') c')
+           (cbn.st (x ++ (l, m) :: y) m')
+→ eq_terms m (cem.conf (x' ++ (l, cem.cl c e) :: y') c).
+intros. destruct H. destruct H0. destruct H1. unfold eq_heaps in H2. apply
+related_lists_inf in H2. destruct H2. assumption. unfold not. split; intros;
+destruct H3; destruct H3; destruct x0; destruct H4; subst; destruct H0;
+destruct H4; unfold domain in H4; rewrite map_app in H4; simpl in H4; apply
+unique_app_comm in H4; inversion H4; apply not_in_app in H9; destruct H9; apply
+in_map with (B:=nat) (f:=@fst nat expr.tm) in H3; simpl in H3. specialize (H11
+H3). inversion H11. specialize (H9 H3). inversion H9. Qed. 
+
+Lemma eq_confs_var1 : ∀ Φ Ψ x t e, 
+  eq_confs (cem.conf Φ (cem.close t e)) 
+           (cbn.st Ψ (expr.var x)) → 
+  ∃ v, t = db.var v.
+intros. inversion H. destruct H1. destruct H2. inversion H2. destruct t. exists
+n. reflexivity. inversion H5. 
+destruct ((fix cte' (t0 : lgexpr) : option lgexpr :=
+  match t0 with
+  | gvar v => (gvar ∘ fst (B:=cem.closure)) <$> cem.clu v e Φ
+  | lvar v => Some (lvar v)
+  | lam b => lam <$> cte' b
+  | app m n => app <$> cte' m <*> cte' n
+  end) (cte t 1)); inversion H6. simpl in H5. 
+destruct ((fix cte' (t : lgexpr) : option lgexpr :=
+  match t with
+  | gvar v => (gvar ∘ fst (B:=cem.closure)) <$> cem.clu v e Φ
+  | lvar v => Some (lvar v)
+  | lam b => lam <$> cte' b
+  | app m n => app <$> cte' m <*> cte' n
+  end) (cte t1 0)); 
+destruct ((fix cte' (t : lgexpr) : option lgexpr :=
+  match t with
+  | gvar v => (gvar ∘ fst (B:=cem.closure)) <$> cem.clu v e Φ
+  | lvar v => Some (lvar v)
+  | lam b => lam <$> cte' b
+  | app m n => app <$> cte' m <*> cte' n
+  end) (cte t2 0)); inversion H5. Qed.
+
+Lemma eq_confs_lam1 : ∀ Φ Ψ x b t e, 
+  eq_confs (cem.conf Φ (cem.close t e)) 
+           (cbn.st Ψ (expr.abs x b)) → 
+  ∃ b, t = db.lam b.
+intros. inversion H. destruct H1. destruct H2. inversion H2. destruct t.
+inversion H5. destruct (cem.clu (n-0) e Φ); inversion H6. 
+exists t. reflexivity. simpl in H5.
+destruct ((fix cte' (t : lgexpr) : option lgexpr :=
+  match t with
+  | gvar v => (gvar ∘ fst (B:=cem.closure)) <$> cem.clu v e Φ
+  | lvar v => Some (lvar v)
+  | lam b => lam <$> cte' b
+  | app m n => app <$> cte' m <*> cte' n
+  end) (cte t1 0)); 
+destruct ((fix cte' (t : lgexpr) : option lgexpr :=
+  match t with
+  | gvar v => (gvar ∘ fst (B:=cem.closure)) <$> cem.clu v e Φ
+  | lvar v => Some (lvar v)
+  | lam b => lam <$> cte' b
+  | app m n => app <$> cte' m <*> cte' n
+  end) (cte t2 0)); inversion H5. Qed.
+
+Lemma eq_confs_app1 : ∀ Φ Ψ m n t e, 
+  eq_confs (cem.conf Φ (cem.close t e)) 
+           (cbn.st Ψ (expr.app m n)) → 
+  ∃ m n, t = db.app m n.
+intros. inversion H. destruct H1. destruct H2. inversion H2. destruct t. 
+inversion H5. destruct (cem.clu (n0-0) e Φ); inversion H6. 
+simpl in H5.
+destruct ((fix cte' (t0 : lgexpr) : option lgexpr :=
+  match t0 with
+  | gvar v => (gvar ∘ fst (B:=cem.closure)) <$> cem.clu v e Φ
+  | lvar v => Some (lvar v)
+  | lam b => lam <$> cte' b
+  | app m n => app <$> cte' m <*> cte' n
+  end) (cte t 1)); inversion H5. 
+exists t1, t2. reflexivity. Qed.
+
+Lemma map_eq_app {a b} : ∀ xs ys zs (f:a→b), map f xs = ys ++ zs → ∃ ys' zs', 
+  xs = ys' ++ zs' ∧ ys = map f ys' ∧ zs = map f zs'. 
+induction xs; intros. simpl in H. symmetry in H. apply app_eq_nil in H. destruct
+H. subst. exists nil, nil. split. reflexivity. split; reflexivity. destruct ys.
+destruct zs. inversion H. inversion H. subst. simpl in H. specialize (IHxs nil
+(map f xs) f eq_refl). destruct IHxs. destruct H0. exists nil, (a0::xs). auto.
+simpl in H. inversion H. subst. apply IHxs in H2. destruct H2. destruct H0.
+destruct H0. destruct H1. subst. exists (a0::x), x0. auto. Qed. 
+
+Lemma eq_heaps_app1 : ∀ Φ Ψ Υ x M, eq_heaps Υ (Φ ++ (x, M) :: Ψ) → 
+                            ∃ Φ' Ψ' c e, Υ = Φ' ++ (x,cem.cl c e) :: Ψ' 
+                                       ∧ eq_terms M (cem.conf Υ c).
+intros. unfold eq_heaps in H. apply (related_lists_in' _ _ _ (x,M)) in H.
+destruct H. destruct H. destruct x0. destruct c. destruct H0. subst. apply
+in_split in H. destruct H. destruct H. exists x0, x1, c, n0. split; auto. apply
+in_inf. Qed.
+
+Lemma lookup_env {A} : ∀ Φ Ψ x (v:A), unique (domain (Ψ ++ (x, v) :: Φ)) → lookup x
+(Ψ ++ (x, v) :: Φ) = Some v. 
+intros. set (heap:=Ψ ++ (x,v) :: Φ). assert (heap = Ψ ++ (x, v) :: Φ).
+reflexivity. rewrite <- H0 in H. apply unique_domain_lookup. assumption. exists
+Ψ, Φ. assumption. Qed. 
+
+Lemma unique_clu_clo : ∀ Φ Ψ x c c' v e en, unique (domain (Ψ ++ (x, cem.cl c e) :: Φ)) → 
+  cem.clu v en (Ψ ++ (x, cem.cl c e) :: Φ) = Some (x, c') → c = c'. 
+induction v; intros. simpl in H0. destruct (lookup en (Ψ ++ (x, cem.cl c e) ::
+Φ)) eqn:lu. destruct c0. inversion H0. subst. apply lookup_env in H. rewrite H
+in lu. inversion lu. reflexivity. inversion H0. simpl in H0. destruct (lookup en
+(Ψ ++ (x, cem.cl c e) :: Φ)) eqn:lue. destruct c0. apply IHv in H0. assumption.
+assumption. inversion H0. Qed. 
+
+Inductive cem_reachable (h : cem.heap) : nat → cem.closure → Prop := 
+  | rcemi : ∀ i c l e t, cem.clu i e h = Some (l, c) → cem_reachable h l (cem.close t e)
+  | rcemtran : ∀ x i c l e t l', cem.clu i x h = Some (l, c) →
+                          cem_reachable h l' c → cem_reachable h l' (cem.close t e).
+
+Definition cem_acyclic (Φ : cem.heap) : Prop := forevery Φ (λ x, 
+  match x with (l, cem.cl c l') => ¬ cem_reachable Φ l c end). 
+
+
+(*
+Lemma cbn_unreachable_step : ∀ l Φ Ψ t v, unique (domain Φ) → cbn.step (cbn.st Φ
+t) (cbn.st Ψ v) → In l (domain Φ) → ¬ cbn_reachable Φ l t → (¬ cbn_reachable Ψ l
+v ∧ ∀ t', ¬ cbn_reachable Φ l t' → ¬ cbn_reachable Ψ l t'). 
+(*Var*)
+intros l Φ Ψ t v ud H. prep_induction H. induction H; simpl; intros.
+specialize (IHstep l Φ0 (Υ' ++ (x, M) :: Φ') M v ud). inversion H1. inversion
+H2. subst.  clear H1. clear H2. specialize (IHstep eq_refl eq_refl H0).  assert
+(unique (domain (Υ' ++ (x, M) :: Φ'))). set (st1 := cbn.st (Υ ++ (x, M) :: Φ)
+M).  set (st2 := cbn.st (Υ' ++ (x, M) :: Φ') (expr.abs y N)). apply
+(cbn.unique_step st1 st2). assumption. assumption. destruct IHstep. unfold not.
+intros. apply H3. apply rcbntran' with (x:=x) (e':=M).  simpl. auto. rewrite
+lookup_inf. reflexivity. assumption. assumption. subst. split. apply (not_impl _
+_ H2). intros. apply cbn_dup_irrelevent in H5. apply cbn_reachable_app.
+assumption. apply cbn_reachable_cons. rewrite app_comm_cons. rewrite
+unique_domain_app. assumption. apply cbn_reachable_app. rewrite
+unique_domain_app in H1. inversion H1. subst.  assumption. assumption. rewrite
+domain_inf with (m':=M). assumption. intros. apply H4 in H5. unfold not. intros.
+clear H. clear ud. clear H4. clear H3. clear H0. clear Φ Υ. prep_induction H6; induction
+H6; intros; subst. apply rcbni with (h:=Υ' ++ (x0, M) :: Φ') in H0. apply H5 in
+H0. inversion H0. assert (rcb := rcbntran _ _ _ _ _ H6 H0 H1). ap 
+
+with (q:=¬cbn_reachable (Υ' ++). . specialize (H3
+(rcbntran' _ _ _ _ _ H4 H5 H2)). assumption. intros. unfold not. intros. apply cbn_reachable_app.
+assumption. 
+(*Lam*)
+inversion H2. inversion H1. subst. subst. auto. 
+
+(*App*)
+inversion H2. inversion H3. subst. clear H2. clear H3.  specialize (IHstep1 _ _
+_ _ _ ud eq_refl eq_refl H4). assert (st2u := cbn.unique_step (cbn.st Φ0 L) (cbn.st Ψ
+(expr.abs x N)) ud H0). simpl in st2u.  assert (unique (domain ((x', M) :: Ψ))).
+apply ucons. simpl. unfold fresh' in H.  destruct H.  assumption. assumption.
+assert (In l (domain Ψ)). apply cbn.monotonic_heap in H0. rewrite <- subset_eq
+in H0. apply H0 in H4. simpl in H4. assumption. assert (In l (domain ((x',M)::
+Ψ))). simpl. apply or_intror.  assumption. specialize (IHstep2 l _ _ _ _ H2
+eq_refl eq_refl H6). apply IHstep2. unfold not. intros.  apply
+cbn_unreachable_app in H5. destruct H5.  apply IHstep1 in H5. inversion H7.
+subst. simpl in H2.  inversion H2. subst.  simpl in H6. destruct H6. subst.
+apply H12 in H3.  inversion H3. clear IHstep2.  clear H1. clear H3.  clear st2u.
+assert (expr.fvs (expr.subst x (expr.var x') N) ⊆ (expr.fvs (expr.var x') ++
+remove x (expr.fvs N))). apply expr.subst_subset.  rewrite <- subset_eq in H1.
+apply H1 in H9.  apply in_app_or in H9. destruct H9.  simpl in H3. destruct H3.
+subst. apply H12 in H6. inversion H6. inversion H3.  clear H1.  apply
+expr.fvs_body_remove in H3.  apply rcbni with (h:=Ψ) in H3.  apply H5 in H3.
+assumption. subst. unfold lookup in H10. simpl in H10. destruct
+(beq_nat x0 x') eqn:bx0x. inversion H10. subst. apply beq_nat_true in bx0x.
+subst. 
+
+
+apply H5.
+apply rcbni. simpl. apply in_or_app. apply or_introl.  apply .  rewrite <-
+subset_eq
+in
+rmc.     expr.fvs_lam_dom.  H6. subst. apply H11 in Hsimpl in
+H6. subst. destruct H6. subst. destruct H. apply x0 in
+H3. inversion H3. subst. 
+simpl in H3. destruct H6. subst.
+destruct H.
+unfold isfresh in x0. inversion H3. subst. inversion H6. subst.    
+bn_dup_irrelevent with (l:=l). rewrite domain_inf with (m':=M). assumption. 
+
+destruct
+(eq_nat_dec l x); subst; clear IHstep H0 H H3; induction H1;
+intros; subst. apply rcbni. assumption. apply inf_indomain. 
+Focus 2. intros.
+apply rcbntran with (x:=x) (e':=M). simpl. left. reflexivity. apply
+unique_domain_lookup.  assumption. exists Υ, Φ. reflexivity. assumption. apply
+IHstep in H3. apply not_impl with (q:=cbn_reachable (Υ' ++ (x, M) :: Φ') l
+(expr.abs y N)).  assumption. intros. clear H3 IHstep. apply cbn.unique_step in
+H. simpl in H.  Focus 2. simpl. assumption. apply cbn_reachable_app. apply
+unique_domain_app.  assumption. apply cbn_reachable_app in H1. Focus 2. rewrite
+domain_inf with (m':=M). assumption.  clear H0. clear ud. prep_induction H1.
+induction H1; intros; subst. inversion H1. subst. simpl in H2.
+destruct H2. subst. apply
+rcbni. assumption. simpl. apply or_introl. reflexivity. inversion H1. subst. apply rcbni. assumption.
+simpl. apply or_intror. assumption. subst. unfold lookup in H2. simpl in H2.
+destruct (beq_nat x0 x) eqn:x0x. apply beq_nat_true in x0x. subst. inversion H2.
+subst. apply rcbntran with (x:=x) (e':=expr.abs y N). assumption. rewrite
+lookup_app_unique. apply lookup_env. assumption. apply unique_domain_app.
+assumption. apply util.unique_app. assumption. 3 prep_induction H1.
+induction H1; intros; subst. simpl in H1. destruct H1. subst. apply rcbni.
+assumption. simpl. apply or_introl. reflexivity. apply rcbni. assumption. simpl.
+apply or_intror. auto. prep_induction H1. induction H1; intros; subst.
+apply rcbni. assumption.  rewrite domain_inf with (m':=M) in H0.  assumption.
+apply cbn_reachable_app in H1. Focus 2. rewrite domain_inf with (m':=expr.abs y0
+N) in H3. assumption. inversion H1. subst. simpl in H5. destruct H5. subst.
+apply cbn_reachable_app. unfold domain. rewrite map_app. apply util.unique_app.
+rewrite <- map_app. assumption. destruct (eq_nat_dec x y). subst. apply rcbni.
+assumption. simpl. apply or_introl. reflexivity. apply lookup_not_inf with
+(a:=expr.abs y0 N) in n
+.   assumption.
+simpl. induction ewrite unique_ induction H1. simpl in H2. destruct H2. subst. H1. subst.
+simpl in H5. destruct H5. substinversion H1. subst.  apply rcbntran with (x:=x)
+(e':=e'). assumption. destruct (eq_nat_dec x x0).
+subst. rewrite domain_inf with (m':=expr.abs y0 N) in H3. apply lookup_env in
+H3.   rewrite H3 in H0. inversion H0. subst. 
+clear IHcbn_reachable. . subst. apply rcbni. destruct
+(eq_nat_dec y x0).  subst.  subst. rewrite lookup_env in H0. clear
+IHcbn_reachable.  inversion H0. subst.
+clear H0.   
+assumption. assumption. assumption. reflexivity.  reflexivity.  rewrite
+domain_inf with (m':=M). assumption. assumption. simpl. assumption. apply
+rcbntran with (x:=x) (e':=e'). assumption.  apply lookup_app in H0. destruct H0.
+apply lookup_app. left. assumption.  destruct H0. apply lookup_app. right.
+split. assumption. unfold lookup. simpl.  rewrite <- beq_nat_false_iff in n.
+rewrite n. unfold lookup in H2. simpl in H2.  rewrite n in H2. assumption. apply
+IHcbn_reachable with (N0:=N) (y1:=y) (Φ:=Φ) (Υ:=Υ). assumptio 
+lookup_total.  . . . .   . . indomain in H0.    .  .  . . .  . apply IHstep. assumption. inversion H1. subst.  clear H1.
+assert (H':= H). apply (cbn.unique_step (cbn.st (Υ ++ (x, M) :: Φ) M) (cbn.st
+(Υ' ++ (x, M) :: Φ') (expr.abs y N)) ud) in H. simpl in ud. inversion H2. subst.
+rewrite replace_inf in IHstep.  specialize (IHstep eq_refl eq_refl H0). assert
+(¬ cbn_reachable (Υ ++ (x, M) :: Φ) l M). unfold not. intros. apply rcbntran
+with (x:=x) (e:=expr.var x) in H1. apply H3 in H1. assumption. simpl. left.
+reflexivity. apply unique_domain_lookup. assumption. exists Υ, Φ. reflexivity.
+apply IHstep in H1. unfold not. intros. induction H4; simpl;
+intros; subst. rewrite domain_inf with (m':=M) in H5. specialize (H1
+(rcbni _ _ _ H4 H5)). assumption. apply IHcbn_reachable. assumption. assumption.
+intros. clear H2. destruct (eq_nat_dec x x0); subst. simpl in H. rewrite
+domain_inf with (m':=t) in H. apply lookup_env in H. apply (not_impl _ _ _ H1). specialize (IHcbn_reachable
+H0 H3). specialize (H1 (rcbntran _ _ _ _ _ H4 H5specialize (. simpl in IHcbn_reachable. clear H6. specialize
+(H7 (rcbntran _ _ _ _ _ H H0 H4)).  specialize
+(IHcbn_reachable M N y x0 Φ Υ Φ' Υ' H1 ud H2 H3 H'). 
+in H1. apply IHcbn_reachable in . apply IHcbn_reachable; try assumption.
+intros. apply IHstep in H7. rewrite domain_inf
+with (m':=M in specialize (H7
+(rcbntran _ _ _ _ _ H4 H5 H6)). specialize (H3
+(rcbntran _ x _ (expr.var x) _ _)). 
+unfold not in H3. specialize (
+not. intros. induction H1. rewrite domain_inf with (m' := M) in H4. 
+inversion H3. intros.
+simpl in H.  
+(cbn_reachable (Υ ++ (x, M) :: Φ) l (expr.var x)). assert (
+
+
 Lemma eq_confs_step1 : ∀ ce cb cb', eq_confs ce cb → cbn.step cb cb' → ∃ ce',
   cem.step ce ce' ∧ eq_confs ce' cb'. 
-intros. generalize dependent ce. induction H0; intros; subst. destruct H.
-destruct H1. destruct ce. destruct H2. unfold eq_terms in H2. simpl in H2.
-destruct st_clos0. destruct clos_tm. simpl in H2. destruct (cem.clu (n - 0)
+intros. prep_induction H0. induction H0; intros. inversion H. destruct H2.
+destruct ce. destruct H3. assert (H4':=H4). apply eq_heaps_app1 in H4. destruct
+H4. destruct H4.  destruct H4. destruct H4. destruct H4. subst. assert
+(H1':=H1). apply cem.well_formed_inf in H1. inversion H. destruct H6. destruct
+H7. destruct st_clos0. inversion H7. apply eq_confs_var1 in H. destruct H.
+subst. simpl in H10. rewrite <- minus_n_O in H10. Focus 1. destruct (cem.clu x4 clos_env
+(x0 ++ (x, cem.cl x2 x3) :: x1)) eqn:lue. Focus 2. inversion H10. simpl in H10.
+inversion H10. destruct p. simpl in H10. unfold compose in H10. simpl in H10.
+inversion H10. subst. clear H10 H11. assert (lue':=lue). apply unique_clu_clo in
+lue. Focus 2. destruct H4. destruct H4. assumption. subst. clear H4.  simpl
+in H7. clear H3.  clear H4'. simpl in H5.  apply cbn.well_formed_app in H2.
+specialize (IHstep (cem.conf (x0 ++ (n, cem.cl c x3) :: x1) c) (conj H1 (conj H2 (conj H5
+H8)))).  destruct IHstep.  destruct H. simpl in *. destruct x. destruct
+st_clos0.  inversion H3. destruct H9. destruct H10. apply eq_heaps_app1 in H11.
+destruct H11. destruct H11. destruct H11. destruct H11. destruct H11. subst.
+assert (H3':=H3). apply eq_confs_lam1 in H3. destruct H3. subst.  exists
+(cem.conf (x ++ (n, cem.cl (cem.close (db.lam x7) clos_env0) x3) :: x2)
+(cem.close (db.lam x7) clos_env0)). 
+
+assert (c = x5). inversion H5. inversion
+H12. rewrite H11 in H13. destruct c eqn:ce. destruct x5 eqn:x5e.  rewrite <- x5e
+in H13. rewrite <- ce in H13. destruct clos_tm. destruct clos_tm0. simpl in H13.
+destruct (cem.clu (n0 - 0) clos_env2 (x ++ (n, cem.cl x5 x6):: x2)) eqn:clue1. .  (x0 destruct (cem.clu v clos_env1 (x0 ++
+(n, cem.cl c x3) :: x1)) eqn:clu.  induction H12. destruct o
+eqn:o'. subst.    split. Focus 1. apply cem.Id.
+assumption.  assumption. unfold
+eq_terms in H7. i
+
+assumption. apply cem.Id. assumption. 
+apply eq_confs_lam1 in Hdestruct st_clos0.  apply eq_confs_var1 in H. destruct H. subst.
+inversion H6. destruct H7. destruct x4. destruct H8.
+destruct st_clos0. apply eq_confs_lam1 in H6. destruct H6. subst. clear H5.
+assert (H9':=H9). apply eq_heaps_app1 in H9. destruct H9. destruct H5. destruct
+H5. destruct H5.  destruct H5. subst. clear H3. clear H6. clear H2. clear H1.
+clear H4'. apply cem.well_formed_inf' in H. apply cbn.well_formed_app' in H7.
+unfold eq_heaps in H4.   split. apply cem.Id. 
+simpl. destruct H1'. simpl in H1. destruct H1. destruct H1. destruct H1.
+destruct H1.  split. apply
+cem.Id. simpl in H7.
+exists cem.conf apply (related_lists_in' _ _ _ (x,M)) in H9'. destruct
+H9'. destruct H1. destruct x10. destruct c. destruct H2. subst. destruct H4.
+destruct H4.  destruct x0. destruct c.  destruct H5.  subst. unfold eq_terms in
+H3. inversion H3. apply in_split in H4. destruct H4. destruct H4. subst. assert
+(H1':=H1).  apply cem.well_formed_inf in H1.  assert (H2':=H2). apply
+cbn.well_formed_app in
+H2.  unfold eq_confs in IHstep at 1.  specialize (IHstep (cem.conf (x0 ++ (x,
+cem.cl c n0) :: x1) c) (conj H1 (conj H2 (conj H6 H4')))). destruct IHstep.
+destruct H4. destruct x2. assert (H':=H). destruct st_clos0. apply eq_confs_var1
+in H'.  destruct H'. subst. assert (H5':=H5). destruct st_clos1. apply
+eq_confs_lam1 in H5'.  destruct H5'.  subst.  assert (mono:=H4). apply
+cem.monotonic_heap in mono.  rewrite <- subset_eq in mono.  unfold subset' in
+mono. specialize (mono _ (inf_indomain _ _ _ _)). apply in_split in mono.
+destruct mono. destruct H8.  simpl in H8. unfold domain in H8.  apply map_eq_app
+in H8. destruct H8. destruct H8. destruct H8. destruct H9.  destruct x7.
+inversion H10. inversion H10. subst. clear H10. destruct p. simpl. simpl in H4.
+exists (cem.conf (x6 ++ (n,cem.cl (cem.close (db.lam x3) clos_env0) n0) :: x7)
+(cem.close (db.lam x3) clos_env0)). simpl.  split. apply cem.Id. simpl in H7.
+rewrite <- minus_n_O in H7. destruct (cem.clu x2 clos_env (x0 ++ (n, cem.cl c
+n0) :: x1)) eqn:clue. destruct p. inversion H7. subst. apply clu_inf' in clue.
+destruct clue. destruct H8. destruct H8. apply unique_inf in H8. destruct H7.
+destruct H8. destruct H8. subst. inversion H8. subst. reflexivity. destruct H1.
+destruct H9. assumption. inversion H7. assumption.  in H3.
+inversion H3.  inversion H8. estruct (cem.clu n
 clos_env st_heap0) eqn:clue. destruct p. unfold fmap_option in H2. unfold
-compose in H2. simpl in H2. inversion H2. subst. assert (infe:=clue). apply
-clu_inf' in infe. destruct infe. destruct H4. destruct H4. subst. specialize
-(IHstep (cem.conf (x ++ (n0, cem.cl c x1) :: x0) c)). exists
-(cem.conf (x ++ (n0, cem.cl c x1) :: x0) c). split. apply cem.Id. .   
+compose in H2. simpl in H2. inversion H2. subst.
+(cem.conf (x ++ (n0, cem.cl c x1) :: x0) c). split. assert (eq_confs (x ++ (n0 apply cem.Id. .   
 inversion H5. subst. exists (cem.conf st_heap0 (cem.close (db.var n) clos_env)).
 split. clos_env
 
@@ -307,37 +672,6 @@ Lemma cem_cbn_bisim : strong_bisim cem.configuration cbn.configuration
 Admitted. 
 Qed. 
 
-(*Well formed configurations can be collapsed into a closed deBruijn term*)
-Theorem well_formed_cbn_closed_db : ∃ c, cbn.well_formed c ↔ ∃ e, db.closed e.
-intros. destruct c. induction (expr.fvs t). destruct H. 
-induction h. destruct H. crush. assert (expr.closed t).
-unfold expr.closed. apply util.subset_nil2. assumption. apply dbf. split with
-(x:=t). assumption. destruct a. crush. 
-
-(* Relation idea: replace deBruijn variable with lookup location, which makes
-them equal *)
-
-Inductive state_rel : relation cem.configuration cbn.configuration := 
-  | init : forall t e,
-           deBruijn t e -> 
-           state_rel (cem.st nil (cem.close e 0)) (cbn.st nil t)
-  | step : forall a b a' b',
-           state_rel a b ->
-           cem.step a a' -> 
-           cbn.step b b' ->
-           state_rel a' b'.
-
-Lemma ex1 : state_rel (cem.abs (0) 
-
-Fixpoint subst_cbn_config' vs e : expr.tm := match vs with
-  | nil => e
-  | (x,m)::hs => subst_cbn_config' hs (cbn.subst x m e)
-  end.
-
-Definition subst_cbn_config (st : cbn.configuration) : db.expr := match st with
-  | cbn.st hs e => deBruijn (subst_cbn_config' hs e)
-  end.
-
 Theorem cem_cbn_bisim : bisim state_rel cem.step cbn.step.
 unfold bisim.
 intros. split. 
@@ -347,4 +681,5 @@ intros. split.
   (expr.abs v b))).  apply cbn.Abs. split. assumption. 
     apply init. with (cem.st nil (cem.close (db.lam b') 0))
                     (cbn.st nil (expr.abs v b)).
-                  *)
+
+*)
