expr_db.v
@@ -2,6 +2,7 @@ Require expr.
 Require Import List Datatypes.
 Require Import Arith.Peano_dec.
 Require Import db util.
+Require Import Unicode.Utf8. 
 
 (* Compiles standard expressions to terms with deBruijn indices *)
 Fixpoint db (t : expr.tm) (env : Map nat nat) : option tm := match t with 
@@ -22,7 +23,45 @@ Fixpoint db (t : expr.tm) (env : Map nat nat) : option tm := match t with
     end
   end.
 
-(* We say two expressions are alpha equivalent if they compile to the same
-deBruijn term *)
-Definition alpha_equiv (t1 t2 : expr.tm) : Prop := db t1 = db t2.
+Lemma expr_closed_under_db: ∀ t xs, expr.fvs t ⊆ domain xs → {e | db t xs = Some e}.
+intros t. induction t; intros; simpl in H. destruct H. simpl.
+apply in_domain_lookup in H.  destruct H. rewrite e. exists (db.var x).
+reflexivity. 
+
+rewrite app_subset_and in H. destruct H. apply IHt1 in H. apply IHt2 in H0.
+destruct H.  destruct H0. simpl. rewrite e. rewrite e0. exists (db.app x x0).
+reflexivity.   
+
+simpl in H. rewrite <- subset_remove_cons in H. rewrite <- domain_fmap with
+(f:=S) in H.  specialize (IHt ((n,0)::map (fmap S) (xs))). simpl in IHt.  apply
+IHt in H. simpl. destruct H. rewrite e. exists (db.lam x). reflexivity. Qed.
+
+Lemma expr_db_closed_under : ∀ t xs e, db t xs = Some e → expr.fvs t ⊆ domain xs. 
+intros t. induction t; intros; simpl in H.
+
+destruct (lookup n xs) eqn:Heqo. apply lookup_domain in Heqo. simpl. split;
+auto. inversion H. 
+
+simpl. destruct (db t1 xs) eqn:Heqo. destruct (db t2 xs)
+eqn:Heqo0. apply IHt1 in Heqo. apply IHt2 in Heqo0. rewrite app_subset_and; 
+split; auto. inversion H. inversion H. 
+
+specialize (IHt ((n,0)::map (fmap S) xs)). destruct (db t ((n,0)::map (fmap S)
+xs)) eqn:Heqo. inversion H. subst. symmetry in Heqo. specialize (IHt t0
+eq_refl). simpl. simpl in IHt. rewrite domain_fmap in IHt. rewrite <-
+subset_remove_cons.  assumption.  inversion H. Qed.
+
+Lemma expr_db_closed : ∀ t e xs, db t xs = Some e → db.fvs e ⊆ codomain xs. 
+intros t. induction t; intros. inversion H. destruct (lookup n xs). inversion
+H1. subst. simpl. split; auto. unfold codomain. inversion H. remember (lookup n
+xs). destruct o. symmetry in Heqo. apply lookup_codomain in Heqo. inversion H2.
+subst. assumption. inversion H2. inversion H1. simpl in H. remember (db t1 xs).
+remember (db t2 xs). destruct o. destruct o0. symmetry in Heqo. symmetry in
+Heqo0. apply IHt1 in Heqo. apply IHt2 in Heqo0. inversion H. subst. simpl.
+rewrite app_subset_and. split; auto. inversion H. inversion H. inversion H.
+remember (db t ((n,0) :: map (fmap S) xs)). destruct o. symmetry in Heqo. apply
+IHt in Heqo. inversion H1. subst. simpl. simpl in Heqo. unfold codomain in Heqo.
+rewrite map_map in Heqo. rewrite subset_remove_cons in Heqo. apply subset_map with
+(f:=pred) in Heqo. rewrite map_map in Heqo. simpl. rewrite (map_homo _ _
+snd_fmap) in Heqo. assumption. inversion H1. Qed. 
 
